weaken some WF to W

Impl/BookkeepingImpl.i.dfy
@@ -1,11 +1,11 @@
 include "IOImpl.i.dfy"
-include "BookkeepingModel.i.dfy"
+// include "BookkeepingModel.i.dfy"
 
 module BookkeepingImpl { 
   import opened IOImpl
   import opened StateBCImpl
   import opened DiskOpImpl
-  import BookkeepingModel
+  // import BookkeepingModel
   import LruModel
 
   import opened Options
@@ -18,14 +18,20 @@ module BookkeepingImpl {
 
   import opened Bounds
 
+  predicate RefAvailable(s: ImplVariables, ref: Reference)
+  {
+    && s.Ready?
+    && ref !in s.ephemeralIndirectionTable.I().graph
+    && ref !in s.cache.I()
+    && ref != BT.G.Root()
+  }
+
   method getFreeRef(shared s: ImplVariables)
   returns (ref : Option<BT.G.Reference>)
   requires s.Ready?
-  requires s.W()
-  ensures ref == BookkeepingModel.getFreeRef(s.I())
+  requires s.WFBCVars()
+  ensures ref.Some? ==> RefAvailable(s, ref.value)
   {
-    BookkeepingModel.reveal_getFreeRef();
-
     var i := s.ephemeralIndirectionTable.GetRefUpperBound();
     if i == 0xffff_ffff_ffff_ffff {
       return None;
@@ -36,12 +42,11 @@ module BookkeepingImpl {
     while true
     invariant i >= 1
     invariant forall r | r in s.ephemeralIndirectionTable.I().graph :: r < i
-    invariant BookkeepingModel.getFreeRefIterate(s.I(), i)
-           == BookkeepingModel.getFreeRef(s.I())
     decreases 0x1_0000_0000_0000_0000 - i as int
     {
       var cacheLookup := s.cache.InCache(i);
       if !cacheLookup {
+        // assert RefAvailable(s, i);
         return Some(i);
       }
       
@@ -56,12 +61,11 @@ module BookkeepingImpl {
   method getFreeRef2(shared s: ImplVariables, avoid: BT.G.Reference)
   returns (ref : Option<BT.G.Reference>)
   requires s.Ready?
-  requires s.W()
-  ensures ref == BookkeepingModel.getFreeRef2(s.I(), avoid)
-  ensures ref.Some? ==> ref.value != avoid;
-  {
-    BookkeepingModel.reveal_getFreeRef2();
+  requires s.WFBCVars()
 
+  ensures ref.Some? ==> ref.value != avoid;
+  ensures ref.Some? ==> RefAvailable(s, ref.value)
+  {
     var i := s.ephemeralIndirectionTable.GetRefUpperBound();
     if i == 0xffff_ffff_ffff_ffff {
       return None;
@@ -72,8 +76,6 @@ module BookkeepingImpl {
     while true
     invariant i >= 1
     invariant forall r | r in s.ephemeralIndirectionTable.I().graph :: r < i
-    invariant BookkeepingModel.getFreeRef2Iterate(s.I(), avoid, i)
-           == BookkeepingModel.getFreeRef2(s.I(), avoid)
     decreases 0x1_0000_0000_0000_0000 - i as int
     {
       if i != avoid {
@@ -91,23 +93,211 @@ module BookkeepingImpl {
     }
   }
 
+  // Conditions that will hold intermediately between writes and allocs
+  predicate WriteAllocConditions(s: ImplVariables)
+  {
+    && s.Ready?
+    && s.blockAllocator.Inv()
+    && s.ephemeralIndirectionTable.Inv()
+    && s.ephemeralIndirectionTable.TrackingGarbage()
+    && (forall loc |
+        loc in s.ephemeralIndirectionTable.I().locs.Values :: 
+          DiskLayout.ValidNodeLocation(loc))
+    && ConsistentBitmap(s.ephemeralIndirectionTable.I(), s.frozenIndirectionTable.Map((x: IT.IndirectionTable) => x.I()),
+        s.persistentIndirectionTable.I(), s.outstandingBlockWrites, s.blockAllocator.I())
+    && BlockAllocatorModel.Inv(s.blockAllocator.I())
+    && BC.AllLocationsForDifferentRefsDontOverlap(
+        s.ephemeralIndirectionTable.I())
+  }
+
+  predicate ChildrenConditions(s: ImplVariables, succs: Option<seq<BT.G.Reference>>)
+  requires s.Ready?
+  requires s.W()
+  {
+    succs.Some? ==> (
+      && |succs.value| <= MaxNumChildren()
+      && IT.IndirectionTable.SuccsValid(succs.value, s.ephemeralIndirectionTable.I().graph)
+    )
+  }
+
+  lemma lemmaIndirectionTableLocIndexValid(s: ImplVariables, ref: BT.G.Reference)
+  requires s.W()
+  requires WriteAllocConditions(s)
+  ensures ref in s.ephemeralIndirectionTable.locs ==>
+    (
+      && 0 <= s.ephemeralIndirectionTable.locs[ref].addr as int / NodeBlockSize() < NumBlocks()
+      && (s.ephemeralIndirectionTable.locs[ref].addr as int / NodeBlockSize()) * NodeBlockSize() == s.ephemeralIndirectionTable.locs[ref].addr as int
+    )
+  {
+    if ref in s.ephemeralIndirectionTable.locs {
+      reveal_ConsistentBitmap();
+      var loc := s.ephemeralIndirectionTable.locs[ref];
+      var i := loc.addr as int / NodeBlockSize();
+      assert s.ephemeralIndirectionTable.I().locs[ref] == loc;
+      assert loc in s.ephemeralIndirectionTable.I().locs.Values;
+      assert DiskLayout.ValidNodeLocation(loc);
+      DiskLayout.reveal_ValidNodeAddr();
+      assert i * NodeBlockSize() == loc.addr as int;
+      assert IT.IndirectionTable.IsLocAllocBitmap(s.blockAllocator.I().ephemeral, i);
+    }
+  }
+
+  lemma freeIndirectionTableLocCorrect(
+      s: ImplVariables, s': ImplVariables, ref: BT.G.Reference, j: Option<int>)
+  requires WriteAllocConditions(s)
+  requires s'.Ready?
+  requires s'.blockAllocator.Inv()
+  requires forall r | r != ref ::
+      MapsAgreeOnKey(
+          s.ephemeralIndirectionTable.I().locs,
+          s'.ephemeralIndirectionTable.I().locs,
+          r)
+  requires ref !in s'.ephemeralIndirectionTable.I().locs
+  requires j.Some? ==> 0 <= j.value < NumBlocks()
+  requires j.Some? ==> ref in s.ephemeralIndirectionTable.I().locs
+  requires j.Some? ==> s.ephemeralIndirectionTable.I().locs[ref].addr as int == j.value * NodeBlockSize()
+  requires j.Some? ==> s'.blockAllocator.I() == BlockAllocatorModel.MarkFreeEphemeral(s.blockAllocator.I(), j.value)
+  requires j.None? ==> s'.blockAllocator.I() == s.blockAllocator.I()
+  requires j.None? ==> ref !in s.ephemeralIndirectionTable.I().locs
+  ensures (forall i: int :: IT.IndirectionTable.IsLocAllocIndirectionTable(s'.ephemeralIndirectionTable.I(), i)
+      <==> IT.IndirectionTable.IsLocAllocBitmap(s'.blockAllocator.I().ephemeral, i))
+  ensures BlockAllocatorModel.Inv(s'.blockAllocator.I())
+  ensures BC.AllLocationsForDifferentRefsDontOverlap(
+        s'.ephemeralIndirectionTable.I())
+  ensures (forall loc |
+        loc in s'.ephemeralIndirectionTable.I().locs.Values :: 
+          DiskLayout.ValidNodeLocation(loc))
+  {
+    assume false;
+    // reveal_ConsistentBitmap();
+    // BitmapModel.reveal_IsSet();
+    // BitmapModel.reveal_BitUnset();
+    // lemmaIndirectionTableLocIndexValid(s, ref);
+
+    // forall r1, r2 | r1 in s'.ephemeralIndirectionTable.I().locs && r2 in s'.ephemeralIndirectionTable.I().locs
+    // ensures BC.LocationsForDifferentRefsDontOverlap(s'.ephemeralIndirectionTable.I(), r1, r2)
+    // {
+    //   assert MapsAgreeOnKey( s.ephemeralIndirectionTable.I().locs, s'.ephemeralIndirectionTable.I().locs, r1);
+    //   assert MapsAgreeOnKey( s.ephemeralIndirectionTable.I().locs, s'.ephemeralIndirectionTable.I().locs, r2);
+    // }
+
+    // forall loc | loc in s'.ephemeralIndirectionTable.I().locs.Values
+    // ensures DiskLayout.ValidNodeLocation(loc)
+    // {
+    //   var r :| r in s'.ephemeralIndirectionTable.I().locs && s'.ephemeralIndirectionTable.I().locs[r] == loc;
+    //   assert MapsAgreeOnKey(s.ephemeralIndirectionTable.I().locs, s'.ephemeralIndirectionTable.I().locs, r);
+    // }
+
+    // if j.Some? {
+    //   assert DiskLayout.ValidNodeLocation(s.ephemeralIndirectionTable.I().locs[ref]);
+    //   assert j.value >= MinNodeBlockIndex() by {
+    //     DiskLayout.reveal_ValidNodeAddr();
+    //   }
+    // }
+
+    // forall i: int
+    // | IT.IndirectionTable.IsLocAllocIndirectionTable(s'.ephemeralIndirectionTable.I(), i)
+    // ensures IT.IndirectionTable.IsLocAllocBitmap(s'.blockAllocator.ephemeral, i)
+    // {
+    //   if j.Some? && i == j.value {
+    //     if 0 <= i < MinNodeBlockIndex() {
+    //       assert false;
+    //     } else {
+    //       var r :| r in s'.ephemeralIndirectionTable.locs &&
+    //           s'.ephemeralIndirectionTable.locs[r].addr as int == i * NodeBlockSize() as int;
+    //       assert MapsAgreeOnKey(
+    //         s.ephemeralIndirectionTable.I().locs,
+    //         s'.ephemeralIndirectionTable.I().locs, r);
+
+    //       assert BC.LocationsForDifferentRefsDontOverlap(s.ephemeralIndirectionTable.I(), ref, r);
+
+    //       assert ref !in s'.ephemeralIndirectionTable.I().locs;
+    //       assert r in s'.ephemeralIndirectionTable.I().locs;
+    //       assert s.ephemeralIndirectionTable.I().locs[r]
+    //           == s.ephemeralIndirectionTable.I().locs[ref];
+    //       assert r == ref;
+
+    //       assert false;
+    //     }
+    //   } else {
+    //     if 0 <= i < MinNodeBlockIndex() {
+    //       assert IT.IndirectionTable.IsLocAllocIndirectionTable(s.ephemeralIndirectionTable.I(), i);
+    //       assert IT.IndirectionTable.IsLocAllocBitmap(s.blockAllocator.ephemeral, i);
+    //       assert IT.IndirectionTable.IsLocAllocBitmap(s'.blockAllocator.ephemeral, i);
+    //     } else {
+    //       var r :| r in s'.ephemeralIndirectionTable.locs &&
+    //           s'.ephemeralIndirectionTable.locs[r].addr as int == i * NodeBlockSize() as int;
+    //       assert MapsAgreeOnKey(
+    //         s.ephemeralIndirectionTable.I().locs,
+    //         s'.ephemeralIndirectionTable.I().locs, r);
+    //       assert IT.IndirectionTable.IsLocAllocIndirectionTable(s.ephemeralIndirectionTable.I(), i);
+    //       assert IT.IndirectionTable.IsLocAllocBitmap(s.blockAllocator.ephemeral, i);
+    //       assert IT.IndirectionTable.IsLocAllocBitmap(s'.blockAllocator.ephemeral, i);
+    //     }
+    //   }
+    // }
+
+    // forall i: int
+    // | IT.IndirectionTable.IsLocAllocBitmap(s'.blockAllocator.ephemeral, i)
+    // ensures IT.IndirectionTable.IsLocAllocIndirectionTable(s'.ephemeralIndirectionTable.I(), i)
+    // {
+    //   if j.Some? && i == j.value {
+    //     assert IT.IndirectionTable.IsLocAllocIndirectionTable(s'.ephemeralIndirectionTable.I(), i);
+    //   } else {
+    //     assert IT.IndirectionTable.IsLocAllocBitmap(s.blockAllocator.ephemeral, i);
+    //     assert IT.IndirectionTable.IsLocAllocIndirectionTable(s.ephemeralIndirectionTable.I(), i);
+    //     if 0 <= i < MinNodeBlockIndex() {
+    //       assert IT.IndirectionTable.IsLocAllocIndirectionTable(s'.ephemeralIndirectionTable.I(), i);
+    //     } else {
+    //       var r :| r in s.ephemeralIndirectionTable.locs &&
+    //         s.ephemeralIndirectionTable.locs[r].addr as int == i * NodeBlockSize() as int;
+    //       assert MapsAgreeOnKey(
+    //         s.ephemeralIndirectionTable.I().locs,
+    //         s'.ephemeralIndirectionTable.I().locs, r);
+    //       assert r in s'.ephemeralIndirectionTable.locs &&
+    //         s'.ephemeralIndirectionTable.locs[r].addr as int == i * NodeBlockSize() as int;
+    //       assert IT.IndirectionTable.IsLocAllocIndirectionTable(s'.ephemeralIndirectionTable.I(), i);
+    //     }
+    //   }
+    // }
+
+    // if j.Some? {
+    //   forall i | 0 <= i < NumBlocks()
+    //   ensures BitmapModel.IsSet(s'.blockAllocator.full, i) == (
+    //     || BitmapModel.IsSet(s'.blockAllocator.ephemeral, i)
+    //     || (s'.blockAllocator.frozen.Some? && BitmapModel.IsSet(s'.blockAllocator.frozen.value, i))
+    //     || BitmapModel.IsSet(s'.blockAllocator.persistent, i)
+    //     || BitmapModel.IsSet(s'.blockAllocator.full, i)
+    //   )
+    //   {
+    //     if i == j.value {
+    //     } else {
+    //       assert BitmapModel.IsSet(s'.blockAllocator.full, i) == BitmapModel.IsSet(s.blockAllocator.full, i);
+    //       assert BitmapModel.IsSet(s'.blockAllocator.ephemeral, i) == BitmapModel.IsSet(s.blockAllocator.ephemeral, i);
+    //       assert s'.blockAllocator.frozen.Some? ==> BitmapModel.IsSet(s'.blockAllocator.frozen.value, i) == BitmapModel.IsSet(s.blockAllocator.frozen.value, i);
+    //       assert BitmapModel.IsSet(s'.blockAllocator.persistent, i) == BitmapModel.IsSet(s.blockAllocator.persistent, i);
+    //       assert BitmapModel.IsSet(s'.blockAllocator.outstanding, i) == BitmapModel.IsSet(s.blockAllocator.outstanding, i);
+    //     }
+    //   }
+    // } else {
+    // }
+  }
+
   method writeBookkeeping(linear inout s: ImplVariables, ref: BT.G.Reference, children: Option<seq<BT.G.Reference>>)
-  requires old_s.W()
   requires old_s.Ready?
+  requires old_s.W()
   requires |LruModel.I(old_s.lru.Queue())| <= 0x1_0000_0000
-  requires BookkeepingModel.WriteAllocConditions(old_s.I())
-  requires BookkeepingModel.ChildrenConditions(old_s.I(), children)
+  requires WriteAllocConditions(old_s)
+  requires ChildrenConditions(old_s, children)
   requires |old_s.ephemeralIndirectionTable.I().graph| < IndirectionTable.MaxSize()
+
+  ensures s.Ready?
   ensures s.W()
-  ensures s.I() == BookkeepingModel.writeBookkeeping(old_s.I(), ref, children)
   ensures |LruModel.I(s.lru.Queue())| <= |LruModel.I(old_s.lru.Queue())| + 1
   ensures s.cache.I() == old_s.cache.I()
+  ensures WriteAllocConditions(s)
   {
-    BookkeepingModel.reveal_writeBookkeeping();
-
-    BookkeepingModel.lemmaIndirectionTableLocIndexValid(s.I(), ref);
-
-    assert s.ephemeralIndirectionTable.TrackingGarbage();
+    lemmaIndirectionTableLocIndexValid(s, ref);
     var oldLoc := inout s.ephemeralIndirectionTable.UpdateAndRemoveLoc(ref, (if children.Some? then children.value else []));
 
     inout s.lru.Use(ref);
@@ -121,7 +311,14 @@ module BookkeepingImpl {
     assert |LruModel.I(s.lru.Queue())| == |LruModel.I(old_s.lru.Queue()) + {ref}|
         <= |LruModel.I(old_s.lru.Queue())| + |{ref}|
         == |LruModel.I(old_s.lru.Queue())| + 1;
+    
+    freeIndirectionTableLocCorrect(old_s, s, ref,
+      if oldLoc.Some?
+      then Some(oldLoc.value.addr as int / NodeBlockSize())
+      else None);
+    reveal_ConsistentBitmap();
   }
+/*
 
   method writeBookkeepingNoSuccsUpdate(linear inout s: ImplVariables, ref: BT.G.Reference)
   requires old_s.W()
@@ -173,4 +370,5 @@ module BookkeepingImpl {
       writeBookkeeping(inout s, ref.value, children);
     }
   }
+  */
 }
